src/FlatDestCheckComp.v
@@ -1,0 +1,310 @@
+Require Import Common Monads.
+Require Import Metadata.
+Require String.
+Require FlatStop FlatDestCheck.
+Require Import ListLemmas.
+Require Import HigherValue.
+
+Require Import Psatz.
+
+Module A := FlatStop.
+Module B := FlatDestCheck.
+
+Add Printing Constructor A.frame.
+Add Printing Constructor B.frame.
+
+
+Definition compile_expr : A.expr -> B.expr :=
+    let fix go e :=
+        match e with
+        | A.Arg => B.Arg
+        | A.Self => B.Self
+        | A.Var i => B.Var i
+        | A.Deref e off => B.Deref (go e) off
+        end in go.
+
+Definition compile : A.stmt -> B.stmt :=
+    let go_expr := compile_expr in
+    let fix go e :=
+        let fix go_list (es : list A.stmt) : list B.stmt :=
+            match es with
+            | [] => []
+            | e :: es => go e :: go_list es
+            end in
+        match e with
+        | A.Skip => B.Skip
+        | A.Seq s1 s2 => B.Seq (go s1) (go s2)
+        | A.Call dst f a => B.Call dst (go_expr f) (go_expr a)
+        | A.MkConstr dst tag args => B.MkConstr dst tag (map go_expr args)
+        | A.Switch dst cases => B.Switch dst (go_list cases)
+        | A.MkClose dst fname free => B.MkClose dst fname (map go_expr free)
+        | A.Assign dst src => B.Assign dst (go_expr src)
+        end in go.
+
+Definition compile_list :=
+    let go := compile in
+    let fix go_list es :=
+        match es with
+        | [] => []
+        | e :: es => go e :: go_list es
+        end in go_list.
+
+Ltac refold_compile :=
+    fold compile_expr in *;
+    fold compile_list in *.
+
+
+
+Inductive I_expr : A.expr -> B.expr -> Prop :=
+| IArg : I_expr A.Arg B.Arg
+| ISelf : I_expr A.Self B.Self
+| IVar : forall i, I_expr (A.Var i) (B.Var i)
+| IDeref : forall ae be off,
+        I_expr ae be ->
+        I_expr (A.Deref ae off) (B.Deref be off)
+.
+
+Inductive I_stmt : A.stmt -> B.stmt -> Prop :=
+| ISkip :
+        I_stmt A.Skip B.Skip
+| ISeq : forall as1 as2 bs1 bs2,
+        I_stmt as1 bs1 ->
+        I_stmt as2 bs2 ->
+        I_stmt (A.Seq as1 as2) (B.Seq bs1 bs2)
+| ICall : forall dst af aa bf ba,
+        I_expr af bf ->
+        I_expr aa ba ->
+        I_stmt (A.Call dst af aa) (B.Call dst bf ba)
+| IMkConstr : forall dst tag aargs bargs,
+        Forall2 I_expr aargs bargs ->
+        I_stmt (A.MkConstr dst tag aargs) (B.MkConstr dst tag bargs)
+| ISwitch : forall dst acases bcases,
+        Forall2 I_stmt acases bcases ->
+        I_stmt (A.Switch dst acases) (B.Switch dst bcases)
+| IMkClose : forall dst fname afree bfree,
+        Forall2 I_expr afree bfree ->
+        I_stmt (A.MkClose dst fname afree) (B.MkClose dst fname bfree)
+| IAssign : forall dst asrc bsrc,
+        I_expr asrc bsrc ->
+        I_stmt (A.Assign dst asrc) (B.Assign dst bsrc)
+.
+Hint Resolve ISkip.
+
+Inductive I_func : (A.stmt * A.expr) -> (B.stmt * B.expr) -> Prop :=
+| IFunc : forall aret acode bret bcode,
+        I_expr aret bret ->
+        I_stmt acode bcode ->
+        I_func (acode, aret) (bcode, bret).
+
+Inductive I_frame : A.frame -> B.frame -> Prop :=
+| IFrame : forall arg self locals,
+        I_frame (A.Frame arg self locals) (B.Frame arg self locals).
+Hint Constructors I_frame.
+
+Inductive I_cont : A.cont -> B.cont -> Prop :=
+| IkSeq : forall acode ak bcode bk,
+        I_stmt acode bcode ->
+        I_cont ak bk ->
+        I_cont (A.Kseq acode ak)
+               (B.Kseq bcode bk)
+| IkSwitch : forall ak bk,
+        I_cont ak bk ->
+        I_cont (A.Kswitch ak)
+               (B.Kswitch bk)
+| IkReturn : forall aret ak bret bk,
+        I_expr aret bret ->
+        I_cont ak bk ->
+        I_cont (A.Kreturn aret ak)
+               (B.Kreturn bret bk)
+| IkCall : forall dst af ak bf bk,
+        I_frame af bf ->
+        I_cont ak bk ->
+        ~ In dst (keys (A.locals af)) ->
+        ~ In dst (A.cont_all_dests ak) ->
+        disjoint (keys (A.locals af)) (A.cont_all_dests ak) ->
+        I_cont (A.Kcall dst af ak)
+               (B.Kcall dst bf bk)
+| IkStop :
+        I_cont A.Kstop
+               B.Kstop
+.
+
+Inductive I : A.state -> B.state -> Prop :=
+| IRun : forall acode af ak  bcode bf bk,
+        I_stmt acode bcode ->
+        I_frame af bf ->
+        I_cont ak bk ->
+        disjoint (keys (A.locals af)) (A.all_dests acode ++ A.cont_all_dests ak) ->
+        I (A.Run acode af ak)
+          (B.Run bcode bf bk)
+
+| IReturn : forall v ak bk,
+        I_cont ak bk ->
+        I (A.Return v ak)
+          (B.Return v bk)
+.
+
+
+
+Lemma compile_I_expr : forall a b,
+    compile_expr a = b ->
+    I_expr a b.
+induction a;
+intros0 Hcomp; simpl in Hcomp; try rewrite <- Hcomp; refold_compile;
+try solve [econstructor; eauto].
+Qed.
+
+Lemma map_compile_I_expr : forall a b,
+    map compile_expr a = b ->
+    Forall2 I_expr a b.
+induction a;
+intros0 Hcomp; simpl in Hcomp; try rewrite <- Hcomp; refold_compile;
+try solve [econstructor; eauto using compile_I_expr].
+Qed.
+
+Theorem compile_I_stmt : forall a b,
+    compile a = b ->
+    I_stmt a b.
+induction a using A.stmt_rect_mut with
+    (Pl := fun a => forall b,
+        compile_list a = b ->
+        Forall2 I_stmt a b);
+intros0 Hcomp; simpl in Hcomp; try rewrite <- Hcomp; refold_compile;
+try solve [econstructor; eauto using compile_I_expr, map_compile_I_expr].
+Qed.
+
+
+
+Ltac i_ctor := intros; econstructor; simpl; eauto.
+Ltac i_lem H := intros; eapply H; simpl; eauto.
+
+Ltac stk_simpl := compute [
+    A.set  A.arg A.self A.locals
+    B.set  B.arg B.self B.locals
+    ] in *.
+
+Lemma set_I_frame : forall af bf dst v,
+    I_frame af bf ->
+    I_frame (A.set af dst v) (B.set bf dst v).
+intros0 II. invc II.
+stk_simpl. constructor.
+Qed.
+Hint Resolve set_I_frame.
+
+Hint Constructors B.eval.
+
+Lemma eval_sim : forall af ae v bf be,
+    I_frame af bf ->
+    I_expr ae be ->
+    A.eval af ae v ->
+    B.eval bf be v.
+induction ae; intros0 IIframe IIexpr Aeval;
+invc IIframe; invc Aeval; invc IIexpr;
+solve [econstructor; eauto].
+Qed.
+Hint Resolve eval_sim.
+
+Lemma eval_sim_forall : forall af aes vs bf bes,
+    I_frame af bf ->
+    Forall2 I_expr aes bes ->
+    Forall2 (A.eval af) aes vs ->
+    Forall2 (B.eval bf) bes vs.
+first_induction aes; intros0 IIframe IIexpr Aeval;
+invc IIexpr; invc Aeval.
+- eauto.
+- constructor; eauto using eval_sim.
+Qed.
+Hint Resolve eval_sim_forall.
+
+Theorem I_sim : forall AE BE a a' b,
+    Forall2 I_func AE BE ->
+    A.state_dests_ok a ->
+    I a b ->
+    A.sstep AE a a' ->
+    exists b',
+        B.sstep BE b b' /\
+        I a' b'.
+destruct a as [ae af ak | val ak ];
+intros0 Henv Adests II Astep;
+inv Astep; inv II;
+try on >I_stmt, invc;
+try on >I_frame, invc;
+simpl in *; A.refold_all_dests.
+
+- (* Seq *)
+  eexists. split. eapply B.SSeq; eauto.
+  i_ctor. i_ctor.
+    { rewrite app_assoc. auto. }
+
+- (* MkConstr *)
+  eexists. split. eapply B.SConstrDone; eauto.
+    { eapply in_keys_lookup_none. simpl. eauto using disjoint_head_r. }
+  i_ctor.
+    { eapply cons_disjoint_l.
+      - repeat break_and. on _, invc_using disjoint_cons_inv_l. auto.
+      - eapply tail_disjoint_r. eauto. }
+
+- (* MkClose *)
+  eexists. split. eapply B.SCloseDone; eauto.
+    { eapply in_keys_lookup_none. simpl. eauto using disjoint_head_r. }
+  i_ctor.
+    { eapply cons_disjoint_l.
+      - repeat break_and. on _, invc_using disjoint_cons_inv_l. auto.
+      - eapply tail_disjoint_r. eauto. }
+
+- (* MakeCall *)
+  fwd eapply Forall2_nth_error_ex with (xs := AE) as HH; eauto.
+    destruct HH as ([bbody bret] & ? & ?).
+  on >I_func, invc.
+
+  eexists. split. eapply B.SMakeCall; eauto.
+    { eapply in_keys_lookup_none. simpl. eauto using disjoint_head_r. }
+  i_ctor. i_ctor. i_ctor.
+    { repeat break_and. on _, invc_using disjoint_cons_inv_r. auto. }
+    { repeat break_and. on _, invc_using disjoint_cons_inv_l. auto. }
+
+- (* Switchinate *)
+  fwd eapply Forall2_nth_error_ex with (xs := cases) as HH; eauto.  destruct HH as (bcase & ? & ?).
+
+  eexists. split. eapply B.SSwitchinate; eauto.
+  i_ctor. i_ctor.
+    { on _, invc_using disjoint_app_inv_r.
+      eapply disjoint_app_r; [|eauto].
+      eapply A.all_dests_list_disjoint; eauto. }
+
+- (* Assign *)
+  eexists. split. eapply B.SAssign; eauto.
+    { eapply in_keys_lookup_none. simpl. eauto using disjoint_head_r. }
+  i_ctor.
+    { eapply cons_disjoint_l.
+      - repeat break_and. on _, invc_using disjoint_cons_inv_l. auto.
+      - eapply tail_disjoint_r. eauto. }
+
+
+- (* ContSeq *)
+  on >I_cont, inv.
+
+  eexists. split. eapply B.SContSeq; eauto.
+  i_ctor.
+
+- (* ContSwitch *)
+  on >I_cont, inv.
+
+  eexists. split. eapply B.SContSwitch; eauto.
+  i_ctor.
+
+- (* ContReturn *)
+  on >I_cont, inv.
+
+  eexists. split. eapply B.SContReturn; eauto.
+  i_ctor.
+
+- (* ContCall *)
+  on >I_cont, inv.
+
+  eexists. split. eapply B.SContCall; eauto.
+    { eapply in_keys_lookup_none. simpl.
+      on >I_frame, invc. simpl in *. auto. }
+  i_ctor.
+Qed.
+
